src/dafny/beacon/statetransition/ProcessOperations.dfy
@@ -21,14 +21,16 @@ include "../../utils/SeqHelpers.dfy"
 include "../../ssz/Constants.dfy"
 include "../BeaconChainTypes.dfy"
 include "../validators/Validators.dfy"
+include "../validators/ValidatorHelpers.dfy"
 include "../attestations/AttestationsTypes.dfy"
 include "../Helpers.dfy"
 include "../Helpers.s.dfy"
 include "../attestations/AttestationsHelpers.dfy"
 include "ProcessOperations.s.dfy"
+include "ProcessOperations.p.dfy"
 
 /**
- * State transition function for the Beacon Chain.
+ *  Process operations and related components for the Beacon Chain.
  */
 module ProcessOperations {
     
@@ -40,6 +42,7 @@ module ProcessOperations {
     import opened Constants
     import opened BeaconChainTypes
     import opened Validators
+    import opened ValidatorHelpers
     import opened AttestationsTypes
     import opened Helpers
     import opened BeaconHelperSpec
@@ -47,19 +50,24 @@ module ProcessOperations {
     import opened BeaconHelpers
     import opened AttestationsHelpers
     import opened ProcessOperationsSpec
+    import opened ProcessOperationsProofs
     
     
-
     /** 
      *  Process the operations defined by a block body.
      *  
      *  @param  s   A state.
      *  @param  bb  A block body.
      *  @returns    The state obtained after applying the operations of `bb` to `s`.
+     *
+     *  @note       This implementation currently takes several minutes to verify.
+     *              An option to optimise would be to more explicity assert component
+     *              pre and post conditions to speed up verification.
      */
     method process_operations(s: BeaconState, bb: BeaconBlockBody)  returns (s' : BeaconState) 
         requires  |s.validators| == |s.balances|
-        requires minimumActiveValidators(s) //|get_active_validator_indices(s.validators, get_current_epoch(s))| > 0
+        //|get_active_validator_indices(s.validators, get_current_epoch(s))| > 0
+        requires minimumActiveValidators(s) 
         requires isValidBeaconBlockBody(s, bb)
         
         ensures s' == updateOperations(s,bb)
@@ -67,7 +75,6 @@ module ProcessOperations {
         ensures s'.slot == s.slot
         ensures s'.latest_block_header == s.latest_block_header
     {
-
         s':= s;
         var slashed_any := false;
 
@@ -78,45 +85,31 @@ module ProcessOperations {
         assert |s'.validators| == |s'.balances|;
         assert s'.slot == s.slot;
         assert s'.latest_block_header == s.latest_block_header;
+        assert forall j :: i <= j < |bb.proposer_slashings| 
+            ==> s'.validators[bb.proposer_slashings[j].header_1.proposer_index] 
+                == s.validators[bb.proposer_slashings[j].header_1.proposer_index];
 
         while i < |bb.proposer_slashings| 
             decreases |bb.proposer_slashings| - i
 
             invariant 0 <= i <= |bb.proposer_slashings| 
-            
             invariant |s'.validators| ==  |s.validators| 
             invariant s' == updateProposerSlashings(s, bb.proposer_slashings[..i])
-            
             invariant s'.slot == s.slot
             invariant s'.latest_block_header == s.latest_block_header
             
         {
-            //requires 0 <= i < |s| - 1
             assert 1 <= |bb.proposer_slashings|; 
-            //assert 0 <= i < |bb.proposer_slashings| - 1;
             seqInitLast<ProposerSlashing>(bb.proposer_slashings, i);
-            assert bb.proposer_slashings[..i+1] == bb.proposer_slashings[..i] + [bb.proposer_slashings[i]];
-
-            //assert forall j :: i <= j < |bb.proposer_slashings| ==> s'.validators[bb.proposer_slashings[j].header_1.proposer_index] == s.validators[bb.proposer_slashings[j].header_1.proposer_index];
-            
-            //assert bb.proposer_slashings[i].header_1.proposer_index as int < |s'.validators|;
-            //assert !s.validators[bb.proposer_slashings[i].header_1.proposer_index].slashed;
-            //assert s' == updateProposerSlashings(s, bb.proposer_slashings[..i]); 
-            //assert forall j :: 0 <= j < |s.validators| && j !in get_PS_validator_indices(bb.proposer_slashings[..i]) ==> updateProposerSlashings(s, bb.proposer_slashings[..i]).validators[j] == s.validators[j];
-            //assert forall j :: 0 <= j < |s.validators| && j !in get_PS_validator_indices(bb.proposer_slashings[..i]) ==> s'.validators[j] == s.validators[j];
-            
-            helperPSLemma4(bb.proposer_slashings[..i+1]);
-            //assert bb.proposer_slashings[i].header_1.proposer_index as int !in get_PS_validator_indices(bb.proposer_slashings[..i]);
-            //assert !s'.validators[bb.proposer_slashings[i].header_1.proposer_index].slashed;
-            //assert s'.validators[bb.proposer_slashings[i].header_1.proposer_index].activationEpoch <= get_current_epoch(s') < s'.validators[bb.proposer_slashings[i].header_1.proposer_index].withdrawableEpoch;
-            
+            assert bb.proposer_slashings[..i+1] 
+                    == bb.proposer_slashings[..i] + [bb.proposer_slashings[i]];
+            PSHelperLemma3(bb.proposer_slashings[..i+1]);
             s' := process_proposer_slashing(s', bb.proposer_slashings[i]);
-
             i := i + 1;
-
-            
         }
+        fullSeq<ProposerSlashing>(bb.proposer_slashings, i);
         assert bb.proposer_slashings[..i] == bb.proposer_slashings;
+        // store intermediate state to assist with final post condition check
         ghost var s1 := updateProposerSlashings(s, bb.proposer_slashings);
         assert s' == s1;
 
@@ -124,7 +117,6 @@ module ProcessOperations {
         i := 0;
         assert isValidAttesterSlashings(s1, bb);
         assert s' == updateAttesterSlashings(s1, bb.attester_slashings[..i]);
-
         assert |s'.validators| == |s'.balances|;
         assert s'.slot == s.slot;
         assert s'.latest_block_header == s.latest_block_header;
@@ -133,38 +125,27 @@ module ProcessOperations {
             decreases |bb.attester_slashings| - i
 
             invariant 0 <= i <= |bb.attester_slashings| 
-
             invariant |s'.validators| ==  |s.validators| 
-
-            //invariant forall j :: 0 <= j < |bb.attester_slashings[..i]| ==> is_valid_indexed_attestation(updateProposerSlashings(s, bb.proposer_slashings), bb.attester_slashings[j].attestation_1)
-            //invariant forall j :: 0 <= j < |bb.attester_slashings[..i]| ==> is_valid_indexed_attestation(updateProposerSlashings(s, bb.proposer_slashings), bb.attester_slashings[j].attestation_2)
             invariant s' == updateAttesterSlashings(s1, bb.attester_slashings[..i])
-
             invariant s'.slot == s.slot
-            invariant s'.latest_block_header == s.latest_block_header //updateProposerSlashings(s, bb.proposer_slashings).latest_block_header == 
+            invariant s'.latest_block_header == s.latest_block_header
         {
             assert 1 <= |bb.attester_slashings|; 
-            //assert 0 <= i < |bb.attester_slashings| - 1;
             seqInitLast<AttesterSlashing>(bb.attester_slashings, i);
-            assert bb.attester_slashings[..i+1] == bb.attester_slashings[..i] + [bb.attester_slashings[i]];
-            
+            assert bb.attester_slashings[..i+1] 
+                    == bb.attester_slashings[..i] + [bb.attester_slashings[i]];
             valid_indexed_attestation_lemma(s1, s', bb.attester_slashings[i].attestation_1);
             assert is_valid_indexed_attestation(s', bb.attester_slashings[i].attestation_1);
             valid_indexed_attestation_lemma(s1, s', bb.attester_slashings[i].attestation_2);
             assert is_valid_indexed_attestation(s', bb.attester_slashings[i].attestation_2);
-            
-            assert |sorted_intersection(bb.attester_slashings[i].attestation_1.attesting_indices, bb.attester_slashings[i].attestation_2.attesting_indices)| > 0;
-            //assume exists j :: 0 <= j < |sorted_intersection(bb.attester_slashings[i].attestation_1.attesting_indices, bb.attester_slashings[i].attestation_2.attesting_indices)| &&
-            //    is_slashable_validator(s'.validators[sorted_intersection(bb.attester_slashings[i].attestation_1.attesting_indices, bb.attester_slashings[i].attestation_2.attesting_indices)[j]], get_current_epoch(s));
-            // TODO: need to prove at least as many unique slashable validators as there are attester_slashings
-            //      i.e. change the precondition and maybe use a lemma 
-
+            assert |sorted_intersection(bb.attester_slashings[i].attestation_1.attesting_indices, 
+                                        bb.attester_slashings[i].attestation_2.attesting_indices)| > 0;
             s', slashed_any := process_attester_slashing(s', bb.attester_slashings[i]);
             i := i + 1;
-
         }
+        fullSeq<AttesterSlashing>(bb.attester_slashings, i);
         assert bb.attester_slashings[..i] == bb.attester_slashings;
-        ghost var s2 := updateAttesterSlashings(updateProposerSlashings(s, bb.proposer_slashings), bb.attester_slashings);
+        ghost var s2 := updateAttesterSlashings(s1, bb.attester_slashings);
         assert s' == s2;
 
         // process attestations
@@ -179,106 +160,68 @@ module ProcessOperations {
             decreases |bb.attestations| - i
 
             invariant 0 <= i <= |bb.attestations|
-            //invariant s'.eth1_deposit_index == s.eth1_deposit_index + i as uint64
-            
             invariant s' == updateAttestations(s2, bb.attestations[..i])
             invariant |s'.validators| ==  |s.validators| 
             invariant s'.slot == s.slot
             invariant s'.latest_block_header == s.latest_block_header
         {
             assert 1 <= |bb.attestations|; 
-            //assert 0 <= i < |bb.attestations| - 1;
             seqInitLast<Attestation>(bb.attestations, i);
             assert bb.attestations[..i+1] == bb.attestations[..i] + [bb.attestations[i]];
             s':= process_attestation(s', bb.attestations[i]); 
             i := i+1;
-
         }
-
+        fullSeq<Attestation>(bb.attestations, i);
         assert bb.attestations[..i] == bb.attestations;
-        ghost var s3 := updateAttestations(updateAttesterSlashings(updateProposerSlashings(s, bb.proposer_slashings), bb.attester_slashings), bb.attestations);
+        ghost var s3 := updateAttestations(s2, bb.attestations);
         assert s3 == s';
 
-        
         //  process deposits in the beacon block body.
         i := 0;
-        // check process deposit preconditions
         assert s'.eth1_deposit_index == s.eth1_deposit_index;
-        // assume s'.eth1_deposit_index as int +  |bb.deposits| < 0x10000000000000000;
-        // assume total_balances(s3.balances) as nat + total_deposits(bb.deposits) as nat < 0x10000000000000000; 
-
         assert isValidDeposits(s3, bb);
         assert s' == updateDeposits(s3, bb.deposits[..i]);
-
         assert |s'.validators| == |s'.balances|;
         assert s'.slot == s.slot;
         assert s'.latest_block_header == s.latest_block_header;
-
         assert s' == updateDeposits(s3, bb.deposits[..i]);
-        assert total_balances(s'.balances) + total_deposits(bb.deposits[..i]) < 0x10000000000000000 ;
+        assert total_balances(s'.balances) + total_deposits(bb.deposits[..i]) 
+                < 0x10000000000000000;
         
         while i < |bb.deposits| 
             decreases |bb.deposits| - i
 
             invariant 0 <= i <= |bb.deposits|
             invariant s'.eth1_deposit_index == s.eth1_deposit_index + i as uint64
-            
-            invariant total_balances(s3.balances) + total_deposits(bb.deposits[..i]) < 0x10000000000000000 
-            //invariant s'.validators == updateDeposits(s, bb.deposits[..i]).validators
-            //invariant s'.balances == updateDeposits(s, bb.deposits[..i]).balances
-            
-            //invariant total_balances(updateDeposits(s,bb.deposits[..i]).balances) == total_balances(s.balances) + total_deposits(bb.deposits[..i]) < 0x10000000000000000
-            
-            //invariant s'.slot == s.slot 
-            //invariant s'.latest_block_header == s.latest_block_header
-            //invariant s'.block_roots == s.block_roots
-            //invariant s'.state_roots == s.state_roots
-
+            invariant total_balances(s3.balances) + total_deposits(bb.deposits[..i]) 
+                        < 0x10000000000000000 
             invariant |s'.validators| == |s'.balances| 
-            //invariant |s'.validators| <= |s.validators| + i
-            //invariant |s.validators| + i <= VALIDATOR_REGISTRY_LIMIT as int
             invariant s' == updateDeposits(s3, bb.deposits[..i])
             invariant s'.slot == s.slot
             invariant s'.latest_block_header == s.latest_block_header
-            //invariant |bb.deposits[..i]| == i
-
-            //invariant |s'.validators| <= |updateDeposits(s,bb.deposits[..i]).validators| <= |s'.validators| + i 
         {
             assert 1 <= |bb.deposits|; 
-            //assert 0 <= i < |bb.deposits| - 1;
             seqInitLast<Deposit>(bb.deposits, i);
             assert bb.deposits[..i+1] == bb.deposits[..i] + [bb.deposits[i]];
-            //assert total_balances(updateDeposits(s, bb.deposits[..i]).balances) + bb.deposits[i].data.amount as int == total_balances(s.balances) + total_deposits(bb.deposits[..i]) + bb.deposits[i].data.amount as int;
-            //assert total_deposits(bb.deposits[..i]) + bb.deposits[i].data.amount as int == total_deposits(bb.deposits[..i+1]);
-            //assert total_balances(updateDeposits(s, bb.deposits[..i]).balances) + bb.deposits[i].data.amount as int == total_balances(s.balances) + total_deposits(bb.deposits[..i+1]);
-            //assert i + 1  <= |bb.deposits|;
             subsetDepositSumProp(bb.deposits, i+1);
-            //assert total_deposits(bb.deposits[..i+1]) <= total_deposits(bb.deposits);
-            //assert total_balances(updateDeposits(s, bb.deposits[..i]).balances) + bb.deposits[i].data.amount as int < 0x10000000000000000;
-
-            //assert updateDeposit(updateDeposits(s, bb.deposits[..i]),bb.deposits[i]) == updateDeposits(s, bb.deposits[..i+1]);
-            
             s':= process_deposit(s', bb.deposits[i]); 
             i := i+1;
-
         }
         assert i == |bb.deposits|;
         fullSeq<Deposit>(bb.deposits, i);
         assert bb.deposits[..i] == bb.deposits;
-        ghost var s4 := updateDeposits(updateAttestations(updateAttesterSlashings(updateProposerSlashings(s, bb.proposer_slashings), bb.attester_slashings), bb.attestations), bb.deposits);
+        ghost var s4 := updateDeposits(s3, bb.deposits);
         assert s4 == s';
 
         // process voluntary exits
         i := 0;
         assert isValidVoluntaryExits(s4, bb);
         assert s' == updateVoluntaryExits(s4, bb.voluntary_exits[..i]);
-
         assert s'.slot == s.slot;
         assert s'.latest_block_header == s.latest_block_header;
         assert |s'.validators| == |s'.balances|;
         assert s'.eth1_deposit_index == s.eth1_deposit_index + |bb.deposits| as uint64;
         
-
         while i < |bb.voluntary_exits| 
             decreases |bb.voluntary_exits| - i
 
@@ -287,34 +230,20 @@ module ProcessOperations {
             invariant s'.slot == s.slot
             invariant s'.latest_block_header == s.latest_block_header
         {
-            helperVolExitLemma4(bb.voluntary_exits[..i+1]);
-             assert 1 <= |bb.voluntary_exits|; 
-             //assert 0 <= i < |bb.voluntary_exits| - 1;
+            VEHelperLemma3(bb.voluntary_exits[..i+1]);
+            assert 1 <= |bb.voluntary_exits|; 
             seqInitLast<VoluntaryExit>(bb.voluntary_exits, i);
             assert bb.voluntary_exits[..i+1] == bb.voluntary_exits[..i] + [bb.voluntary_exits[i]];
-            //assert bb.voluntary_exits[i].validator_index as int < |s.validators| <= |s'.validators|;
-            //assert !s'.validators[bb.voluntary_exits[i].validator_index].slashed;
-
-            //assume s'.validators[bb.voluntary_exits[i].validator_index].activationEpoch <= get_current_epoch(s) < s'.validators[bb.voluntary_exits[i].validator_index].withdrawableEpoch;
-            //assume s'.validators[bb.voluntary_exits[i].validator_index].exitEpoch == FAR_FUTURE_EPOCH;
-            //assume get_current_epoch(s) >= bb.voluntary_exits[i].epoch;
-            //assume get_current_epoch(s) >= s'.validators[bb.voluntary_exits[i].validator_index].activationEpoch + SHARD_COMMITTEE_PERIOD ;
-
             s' := process_voluntary_exit(s', bb.voluntary_exits[i]);
             i := i + 1;
-
         }
         assert i == |bb.voluntary_exits|;
         fullSeq<VoluntaryExit>(bb.voluntary_exits, i);
         assert bb.voluntary_exits[..i] == bb.voluntary_exits;
-        ghost var s5 := updateVoluntaryExits(updateDeposits(updateAttestations(updateAttesterSlashings(updateProposerSlashings(s, bb.proposer_slashings), bb.attester_slashings), bb.attestations), bb.deposits), bb.voluntary_exits);
+        ghost var s5 := updateVoluntaryExits(s4, bb.voluntary_exits);
         assert s5 == s';
         assert s' == updateOperations(s,bb);
-
     }
-
-    
-
 
     /**
      *  Process a proposer slashing.
@@ -322,116 +251,90 @@ module ProcessOperations {
      *  @param  s   A state.
      *  @param  ps  A proposer slashing.  
      *  @returns    The state obtained applying `ps` to `s`.
-     *  @todo       Finish implementation of this function.
      */
     method process_proposer_slashing(s: BeaconState, ps : ProposerSlashing)  returns (s' : BeaconState)  
         requires ps.header_1.slot == ps.header_2.slot
         requires ps.header_1.proposer_index == ps.header_2.proposer_index 
         requires ps.header_1 == ps.header_2
-        
         requires ps.header_1.proposer_index as int < |s.validators| 
-        //requires is_slashable_validator(s.validators[ps.header_1.proposer_index], get_current_epoch(s));
         requires !s.validators[ps.header_1.proposer_index].slashed
-        requires s.validators[ps.header_1.proposer_index].activation_epoch <= get_current_epoch(s) < s.validators[ps.header_1.proposer_index].withdrawable_epoch
-
-        
-        //requires s.validators[ps.header_1.proposer_index].exitEpoch == FAR_FUTURE_EPOCH
+        requires s.validators[ps.header_1.proposer_index].activation_epoch 
+                    <= get_current_epoch(s) 
+                    < s.validators[ps.header_1.proposer_index].withdrawable_epoch
         requires |get_active_validator_indices(s.validators, get_current_epoch(s))| > 0
         requires |s.validators| == |s.balances|
         
         ensures s' == updateProposerSlashing(s,ps)
-        //ensures forall i :: 0 <= i < |s.validators|  && i != ps.header_1.proposer_index as int ==> s'.validators[i] == s.validators[i]
     {
-        // header_1 = proposer_slashing.signed_header_1.message
-        // header_2 = proposer_slashing.signed_header_2.message
-
         // # Verify header slots match
-        // assert header_1.slot == header_2.slot
         assert ps.header_1.slot == ps.header_2.slot;
 
-
         // # Verify header proposer indices match
-        // assert header_1.proposer_index == header_2.proposer_index
         assert ps.header_1.proposer_index == ps.header_2.proposer_index;
 
         // # Verify the headers are different
-        // assert header_1 != header_2
         assert ps.header_1 == ps.header_2;
-
 
         // # Verify the proposer is slashable
         var proposer := s.validators[ps.header_1.proposer_index];
-        
-        //assert is_slashable_validator(proposer, get_current_epoch(s));
         assert is_slashable_validator(proposer, get_current_epoch(s));
 
-
-        // # Verify signatures
-        // for signed_header in (proposer_slashing.signed_header_1, proposer_slashing.signed_header_2):
-        //     domain = get_domain(state, DOMAIN_BEACON_PROPOSER, compute_epoch_at_slot(signed_header.message.slot))
-        //     signing_root = compute_signing_root(signed_header.message, domain)
-        //     assert bls.Verify(proposer.pubkey, signing_root, signed_header.signature)
-
-
+        // # Verify signatures is not implemented
         assert ps.header_1.proposer_index as int < |s.validators| ;
         assert get_beacon_proposer_index(s) as int < |s.validators|;
         assert |s.validators| == |s.balances|;
-
-        //assert s.validators[ps.header_1.proposer_index].exitEpoch == FAR_FUTURE_EPOCH;
         assert |get_active_validator_indices(s.validators, get_current_epoch(s))| > 0;
 
-        // the whistleblower_index parameter of slash_validator is None in the spec
-        // as 'None' isn't possible in Dafny, set the parameter to get_beacon_proposer_index(s)
-        // as it would be set to that for 'None' within slash_validator
-
+        // The whistleblower_index parameter of slash_validator is None in the spec.
+        // As 'None' isn't possible in Dafny, set the parameter to get_beacon_proposer_index(s)
+        // as it would be set to that for 'None' within slash_validator.
         s' := slash_validator(s, ps.header_1.proposer_index, get_beacon_proposer_index(s));
     }
 
-    method process_attester_slashing(s: BeaconState, a: AttesterSlashing) returns (s' : BeaconState, flag: bool) 
-        requires forall i :: 0 <= i < |a.attestation_1.attesting_indices| ==> a.attestation_1.attesting_indices[i] as int < |s.validators|
-        requires forall i :: 0 <= i < |a.attestation_2.attesting_indices| ==> a.attestation_2.attesting_indices[i] as int < |s.validators|
+    /**
+     *  Process an attester slashing.
+     *
+     *  @param  s   A state.
+     *  @param  a   An attester slashing.  
+     *  @returns    The state obtained applying `a` to `s`.
+     */
+    method process_attester_slashing(s: BeaconState, a: AttesterSlashing) 
+            returns (s' : BeaconState, flag: bool) 
+        requires forall i :: 0 <= i < |a.attestation_1.attesting_indices| 
+                    ==> a.attestation_1.attesting_indices[i] as int < |s.validators|
+        requires forall i :: 0 <= i < |a.attestation_2.attesting_indices|
+                    ==> a.attestation_2.attesting_indices[i] as int < |s.validators|
         requires |get_active_validator_indices(s.validators, get_current_epoch(s))| > 0
         requires |s.validators| == |s.balances|
-
         requires is_slashable_attestation_data(a.attestation_1.data, a.attestation_2.data)
-
         requires is_valid_indexed_attestation(s, a.attestation_1)
         requires is_valid_indexed_attestation(s, a.attestation_2)
+        requires |sorted_intersection(a.attestation_1.attesting_indices, 
+                                      a.attestation_2.attesting_indices)| 
+                    > 0
 
-        // not sure whether there should be at least one in the intersection???
-        requires |sorted_intersection(a.attestation_1.attesting_indices, a.attestation_2.attesting_indices)| > 0
-
-        // the following should be used when adding a check that slashed_any == true at the end of the method
-        //requires exists i :: 0 <= i < |sorted_intersection(a.attestation_1.attesting_indices, a.attestation_2.attesting_indices)| &&
-        //    is_slashable_validator(s.validators[sorted_intersection(a.attestation_1.attesting_indices, a.attestation_2.attesting_indices)[i]], get_current_epoch(s))
-
-        ensures s' == updateAttesterSlashing(s, sorted_intersection(a.attestation_1.attesting_indices, a.attestation_2.attesting_indices))
-        //ensures flag
+        ensures s' == updateAttesterSlashing(s, 
+                                            sorted_intersection(a.attestation_1.attesting_indices, 
+                                                                a.attestation_2.attesting_indices)
+                                            )
+        //ensures flag is not implemented in this simplified model
     {
         //Double vote
         //(data_1 != data_2 && data_1.target.epoch == data_2.target.epoch) ||
         // Surround vote
         //(data_1.source.epoch < data_2.source.epoch && data_2.target.epoch < data_1.target.epoch)
         assert is_slashable_attestation_data(a.attestation_1.data, a.attestation_2.data);
-        
-        // assert is_valid_indexed_attestation(state, attestation_1)
         // Verify indices are sorted and unique, and at least 1
         assert is_valid_indexed_attestation(s, a.attestation_1);
-
         // assert is_valid_indexed_attestation(state, attestation_2)
         assert is_valid_indexed_attestation(s, a.attestation_2);
 
         s' := s;
         flag := false;
-        
         var i := 0;
-        
         var origState := s;
-        
         var ts := sorted_intersection(a.attestation_1.attesting_indices, a.attestation_2.attesting_indices);
-
         assert forall i :: 0 <= i < |ts| ==> ts[i] as int < |s'.validators|;
-
         assert s' == updateAttesterSlashing(s, ts[..i]);
         
         while i < |ts| 
@@ -441,79 +344,59 @@ module ProcessOperations {
             invariant |s'.validators| == |s'.balances|
             invariant get_current_epoch(s) == get_current_epoch(s')
             invariant |ts| > 0
-            
-            invariant get_active_validator_indices(s.validators, get_current_epoch(s)) == get_active_validator_indices(s'.validators, get_current_epoch(s));
+            invariant get_active_validator_indices(s.validators, get_current_epoch(s)) 
+                        == get_active_validator_indices(s'.validators, get_current_epoch(s));
             invariant |get_active_validator_indices(s'.validators, get_current_epoch(s'))| > 0
             invariant get_beacon_proposer_index(s) == get_beacon_proposer_index(s')
             invariant get_beacon_proposer_index(s') as int < |s'.validators|
             invariant i == |ts[..i]|
-            
             invariant forall j :: 0 <= j < |ts| ==> ts[j] as int < |s'.validators|
             invariant valid_state_indices(s, ts[..i]);
             invariant s' == updateAttesterSlashing(s, ts[..i])
             invariant s'.slot == s.slot
         {
             origState := s';
-            
-            // if (is_slashable_validator(s'.validators[ts[i]], get_current_epoch(s'))) {
-            //     assert (!s'.validators[ts[i]].slashed) && (s'.validators[ts[i]].activationEpoch <= get_current_epoch(s') < s'.validators[ts[i]].withdrawableEpoch);
-            //     slashValidatorPreservesActivateValidators(s', ts[i], get_beacon_proposer_index(s'));
-            //     s' := slash_validator(s', ts[i], get_beacon_proposer_index(s'));
-            //     flag := true;
-            // }
             if (is_slashable_validator(origState.validators[ts[i]], get_current_epoch(origState))) {
-                assert (!origState.validators[ts[i]].slashed) && (origState.validators[ts[i]].activation_epoch <= get_current_epoch(origState) < origState.validators[ts[i]].withdrawable_epoch);
-                slashValidatorPreservesActivateValidators(origState, ts[i], get_beacon_proposer_index(origState));
+                assert (!origState.validators[ts[i]].slashed) 
+                    && (origState.validators[ts[i]].activation_epoch 
+                            <= get_current_epoch(origState) 
+                            < origState.validators[ts[i]].withdrawable_epoch
+                        );
+                slashValidatorPreservesActiveValidators(origState, 
+                                                        ts[i], 
+                                                        get_beacon_proposer_index(origState)
+                                                    );
                 s' := slash_validator(origState, ts[i], get_beacon_proposer_index(origState));
                 flag := true;
-                //slash_validator_lemma(origState, ts[i], get_beacon_proposer_index(origState));
-
-                //assert slash_validator(origState, ts[i], get_beacon_proposer_index(origState)).validators[ts[i]].slashed;
             }
             else {
                   s' := s';
             }
-            //assert is_slashable_validator(origState.validators[ts[i]], get_current_epoch(origState)) ==> flag;
-            //slash_validator_lemma(origState, ts[i], get_beacon_proposer_index(origState));
-            helperIndicesLemma5(ts,i+1);
-            helperIndicesLemma7(ts,i);
+            assert 1 <= |ts|; 
+            seqInitLast<uint64>(ts, i);
             assert ts[..i+1] == ts[..i] + [ts[i]];
-            helperIndicesLemma4(s,ts, i);
             assert origState == updateAttesterSlashing(s, ts[..i]);
             assert s' == updateAttesterSlashingComp(origState, ts[i]);
             assert s' == updateAttesterSlashingComp(updateAttesterSlashing(s, ts[..i]), ts[i]);
             assert valid_state_indices(s, ts);
             assert 0 < i+1 <= |ts|;
-            helperIndicesLemma4(s,ts, i+1);
             assert valid_state_indices(s, ts[..(i+1)]);
             assert |ts[..(i+1)]| != 0;
-            assert updateAttesterSlashing(s, ts[..(i+1)]) == updateAttesterSlashingComp(updateAttesterSlashing(s, ts[..i]), ts[i]);
+            assert updateAttesterSlashing(s, ts[..(i+1)]) 
+                    == updateAttesterSlashingComp(updateAttesterSlashing(s, ts[..i]), ts[i]);
             assert s' == updateAttesterSlashing(s, ts[..(i+1)]);
             i := i+1;
-            helperIndicesLemma4(s,ts, i);
             assert valid_state_indices(s, ts[..i]);
             assert s' == updateAttesterSlashing(s, ts[..i]);
-            
         }
-        // calc ==> {
-        //     exists j :: 0 <= j < |sorted_intersection(a.attestation_1.attesting_indices, a.attestation_2.attesting_indices)| &&
-        //     is_slashable_validator(s.validators[sorted_intersection(a.attestation_1.attesting_indices, a.attestation_2.attesting_indices)[j]], get_current_epoch(s));
-            
-        //     exists j :: 0 <= j < |ts| && is_slashable_validator(s.validators[ts[j]], get_current_epoch(s'));
-
-        //     slashed_any;
-
-        // }
         assert i == |ts|;
-        helperIndicesLemma6(ts, i);
+        fullSeq<uint64>(ts, i);
         assert ts[..i] == ts;
         assert s' == updateAttesterSlashing(s, ts[..i]);
         assert s' == updateAttesterSlashing(s, ts);
-        assert ts == sorted_intersection(a.attestation_1.attesting_indices, a.attestation_2.attesting_indices);
-        //assert s' == updateAttesterSlashing(s, sorted_intersection(a.attestation_1.attesting_indices, a.attestation_2.attesting_indices));
-
+        assert ts == sorted_intersection(a.attestation_1.attesting_indices, 
+                                         a.attestation_2.attesting_indices);
         //assert slashed_any;
-        
     }
 
     /**
@@ -544,20 +427,28 @@ module ProcessOperations {
      *  MIN_ATTESTATION_INCLUSION_DELAY is 1.
      *
      *  Question: what is the invariant for the attestations in a state?
+     *
+     *  Process an attestation.
+     *
+     *  @param  s   A state.
+     *  @param  a   An attestation.  
+     *  @returns    The state obtained applying `a` to `s`.
      */
     method process_attestation(s: BeaconState, a: Attestation) returns (s' : BeaconState)
         requires attestationIsWellFormed(s, a)
         requires |s.current_epoch_attestations| < MAX_ATTESTATIONS as nat * SLOTS_PER_EPOCH as nat 
         requires |s.previous_epoch_attestations| < MAX_ATTESTATIONS as nat * SLOTS_PER_EPOCH as nat 
         requires minimumActiveValidators(s)
+
         ensures s' == updateAttestation(s,a)
         ensures s'.eth1_deposit_index == s.eth1_deposit_index;
-
     {
         // data = attestation.data
         assert get_previous_epoch(s) <= a.data.target.epoch <=  get_current_epoch(s);
         assert a.data.target.epoch == compute_epoch_at_slot(a.data.slot);
-        assert a.data.slot as nat + MIN_ATTESTATION_INCLUSION_DELAY as nat <= s.slot as nat <= a.data.slot as nat + SLOTS_PER_EPOCH as nat;
+        assert a.data.slot as nat + MIN_ATTESTATION_INCLUSION_DELAY as nat 
+                <= s.slot as nat 
+                <= a.data.slot as nat + SLOTS_PER_EPOCH as nat;
         assert a.data.index < get_committee_count_per_slot(s, a.data.target.epoch);
 
         var committee := get_beacon_committee(s, a.data.slot, a.data.index);
@@ -584,7 +475,6 @@ module ProcessOperations {
                 previous_epoch_attestations := s.previous_epoch_attestations + [pending_attestation]
             );
         }
-             
         // # Verify signature
         // Not implemented as part of the simplificiation
         //assert is_valid_indexed_attestation(s', get_indexed_attestation(s', a));
@@ -596,8 +486,7 @@ module ProcessOperations {
      *  @param  s   A state.
      *  @param  d   A deposit.  
      *  @returns    The state obtained depositing of `d` to `s`.
-     *  @todo       Finish implementation of this function.
-     */
+    */
     method process_deposit(s: BeaconState, d : Deposit)  returns (s' : BeaconState)  
         requires |s.validators| + 1 <= VALIDATOR_REGISTRY_LIMIT as int
         requires s.eth1_deposit_index as int + 1 < 0x10000000000000000 
@@ -605,19 +494,11 @@ module ProcessOperations {
         requires total_balances(s.balances) + d.data.amount as int < 0x10000000000000000
 
         ensures s'.eth1_deposit_index == s.eth1_deposit_index + 1
-        //ensures d.data.pubkey !in seqKeysInValidators(s.validators) ==> s'.validators == s.validators + [get_validator_from_deposit(d)]
-        //ensures d.data.pubkey in seqKeysInValidators(s.validators) ==> s'.validators == s.validators 
-        ensures s' == updateDeposit(s,d)
-
-        //ensures |s'.validators| == |s'.balances|        // maybe include in property lemmas
-        //ensures |s.validators| <= |s'.validators| <= |s.validators| + 1 // maybe include in property lemmas
-        //ensures |s.balances| <= |s'.balances| <= |s.balances| + 1 // maybe include in property lemmas
-        //ensures |s'.validators| <= VALIDATOR_REGISTRY_LIMIT
-        
+        ensures s' == updateDeposit(s,d) 
     {
-        // note that it is assumed that all new validator deposits are verified
-        // ie the step # Verify the deposit signature (proof of possession) which is not checked by the deposit contract
-        // is not performed
+        // Note that it is assumed that all new validator deposits are verified.
+        // i.e. the step # Verify the deposit signature (proof of possession), which is not checked 
+        // by the deposit contract, is not performed.
         var pk := seqKeysInValidators(s.validators);
         s' := s.(
                 eth1_deposit_index := (s.eth1_deposit_index as int + 1) as uint64,
@@ -627,60 +508,57 @@ module ProcessOperations {
                                     (s.validators + [get_validator_from_deposit(d)]),
                 balances := if d.data.pubkey in pk then 
                                     individualBalanceBoundMaintained(s.balances,d);
-                                    increase_balance(s,get_validator_index(pk, d.data.pubkey),d.data.amount).balances
+                                    increase_balance(s,
+                                                    get_validator_index(pk, d.data.pubkey),
+                                                    d.data.amount).balances
                                 else 
                                     s.balances + [d.data.amount]
         );
     }
 
-   
-    // Voluntary exits
+    /**
+     *  Process a voluntary exit.
+     *
+     *  @param  s               A state.
+     *  @param  voluntary_exit  A voluntary exit.  
+     *  @returns                The state obtained applying `voluntary_exit` to `s`.
+     */
     method process_voluntary_exit(s: BeaconState, voluntary_exit: VoluntaryExit) returns (s' : BeaconState) 
         requires |s.validators| == |s.balances|
         requires voluntary_exit.validator_index as int < |s.validators|
-        //requires is_active_validator(s.validators[voluntary_exit.validator_index], get_current_epoch(s))
         requires !s.validators[voluntary_exit.validator_index].slashed
-        requires s.validators[voluntary_exit.validator_index].activation_epoch <= get_current_epoch(s) < s.validators[voluntary_exit.validator_index].withdrawable_epoch
-
+        requires s.validators[voluntary_exit.validator_index].activation_epoch 
+                    <= get_current_epoch(s) 
+                    < s.validators[voluntary_exit.validator_index].withdrawable_epoch
         requires s.validators[voluntary_exit.validator_index].exitEpoch == FAR_FUTURE_EPOCH
         requires get_current_epoch(s) >= voluntary_exit.epoch
-        requires get_current_epoch(s) >= s.validators[voluntary_exit.validator_index].activation_epoch + SHARD_COMMITTEE_PERIOD 
+        requires get_current_epoch(s) 
+                    >= s.validators[voluntary_exit.validator_index].activation_epoch + SHARD_COMMITTEE_PERIOD 
         
         ensures s' == updateVoluntaryExit(s, voluntary_exit)
     {
         var validator := s.validators[voluntary_exit.validator_index];
 
-        // NOTE: If any of the spec asserts fail then the state is unchanged and the voluntary exit not implemented
+        // Note if any of the spec asserts fail then the state is unchanged 
+        // and the voluntary exit is not implemented.
 
         // # Verify the validator is active
-        //assert is_active_validator(validator, get_current_epoch(s)); 
         assert is_active_validator(validator, get_current_epoch(s));
 
         // # Verify exit has not been initiated
-        // assert validator.exit_epoch == FAR_FUTURE_EPOCH; 
         assert validator.exitEpoch == FAR_FUTURE_EPOCH;
 
         // # Exits must specify an epoch when they become valid; they are not valid before then
-        // assert get_current_epoch(state) >= voluntary_exit.epoch; 
         assert get_current_epoch(s) >= voluntary_exit.epoch;
 
         // # Verify the validator has been active long enough
-        // assert get_current_epoch(state) >= validator.activation_epoch + SHARD_COMMITTEE_PERIOD; 
         assert get_current_epoch(s) >= validator.activation_epoch + SHARD_COMMITTEE_PERIOD;
 
         // # Verify signature
-        // Note: Not implemented as this stage
-        // domain = get_domain(state, DOMAIN_VOLUNTARY_EXIT, voluntary_exit.epoch)
-        // signing_root = compute_signing_root(voluntary_exit, domain)
-        // assert bls.Verify(validator.pubkey, signing_root, signed_voluntary_exit.signature)
-
+        // Not implemented as part of the simplificiation.
+        
         // # Initiate exit
         s' := initiate_validator_exit(s, voluntary_exit.validator_index);
     }
-
-
-    
-
-
 
 }
